Some minor, mostly cosmetical, refactoring

Taylor_Models.thy
@@ -12,13 +12,13 @@ section \<open>Multivariate Taylor Models\<close>
 
 subsection \<open>Computing interval bounds on arithmetic expressions\<close>
 
-fun compute_bound :: "nat \<Rightarrow> floatarith \<Rightarrow> float interval list \<Rightarrow> float interval option"
-where "compute_bound prec f I = (case approx prec f (map (Some o proc_of) I) of Some (a, b) \<Rightarrow> (if a \<le> b then Some (Ivl a b) else None) | _ \<Rightarrow> None)"
+fun compute_bound_fa :: "nat \<Rightarrow> floatarith \<Rightarrow> float interval list \<Rightarrow> float interval option"
+where "compute_bound_fa prec f I = (case approx prec f (map (Some o proc_of) I) of Some (a, b) \<Rightarrow> (if a \<le> b then Some (Ivl a b) else None) | _ \<Rightarrow> None)"
 
-lemma compute_bound_correct:
+lemma compute_bound_fa_correct:
 fixes i::"real list"
 assumes "i all_in I"
-assumes "Some ivl = compute_bound prec f I"
+assumes "Some ivl = compute_bound_fa prec f I"
 shows "interpret_floatarith f i \<in> set_of ivl"
 proof-
   have "\<forall>n < length I. \<exists>a b. I!n = Ivl a b \<and> a \<le> b"
@@ -82,7 +82,7 @@ proof-
       show False
         proof(cases "approx prec f (map Some (zip a b))")
           assume assm: "approx prec f (map Some (zip a b)) = None"
-          from assms(2)[unfolded compute_bound.simps I_def]
+          from assms(2)[unfolded compute_bound_fa.simps I_def]
           show "False"
             unfolding domain_simp
             by (simp add: assm case_prod_beta comp_def)
@@ -90,7 +90,7 @@ proof-
           fix ab' assume assm: "approx prec f (map Some (zip a b)) = Some ab'"
           then obtain a' b' where ab'_def: "ab' = (a', b')" by fastforce
           hence "(a', b') \<noteq> (l, u)" using contr_assm assm by auto
-          from assms(2)[unfolded compute_bound.simps I_def] this assm
+          from assms(2)[unfolded compute_bound_fa.simps I_def] this assm
           show False
             unfolding domain_simp
             apply(cases "a' \<le> b'")
@@ -179,13 +179,13 @@ subsection \<open>Interval bounds for taylor models\<close>
 fun compute_bound_poly :: "float poly \<Rightarrow> float interval list \<Rightarrow> float list \<Rightarrow> float interval"
 where "compute_bound_poly p I a = (
          Ipoly (list_op op- I a) p
-         (*let Ds = split_domain (\<lambda>x a. [Ivl (lower x) 0, Ivl 0 (upper x)]) (list_op op- I a) a;
+         (*let Ds = split_domain (\<lambda>x. [Ivl (lower x) 0, Ivl 0 (upper x)]) (list_op op- I a);
              S = map (\<lambda>d. Ipoly d (p :: float interval poly)) Ds
          in interval_list_union S*)
        )"
 
-fun compute_bound_tm :: "taylor_model \<Rightarrow> float interval list \<Rightarrow> float list \<Rightarrow> float interval"
-where "compute_bound_tm (TaylorModel p e) I a = compute_bound_poly p I a + e"
+fun compute_bound_tm :: "float interval list \<Rightarrow> float list \<Rightarrow> taylor_model \<Rightarrow> float interval"
+where "compute_bound_tm I a (TaylorModel p e) = compute_bound_poly p I a + e"
 
 lemma compute_bound_poly_correct:
 fixes p::"float poly"
@@ -228,7 +228,7 @@ lemma compute_bound_tm_correct:
 fixes I :: "float interval list" and x :: "real list" and f :: "real list \<Rightarrow> real"
 assumes "valid_tm I a f t"
 assumes "x all_in I"
-shows "f x \<in> set_of (compute_bound_tm t I a)"
+shows "f x \<in> set_of (compute_bound_tm I a t)"
 proof-
   obtain p l u where t_decomp: "t = TaylorModel p (Ivl l u)"
     by (metis interval_exhaust taylor_model.exhaust)
@@ -240,7 +240,7 @@ proof-
       \<in> set_of (Ivl l u)"
       by auto
   
-  show "f x \<in> set_of (compute_bound_tm t I a)"
+  show "f x \<in> set_of (compute_bound_tm I a t)"
     using set_of_add_mono[OF compute_bound_poly_correct[OF valid(1) assms(2) \<open>a all_in I\<close>] valid(3)]
     by (simp add: t_decomp)
 qed
@@ -250,7 +250,7 @@ fixes I :: "float interval list" and x :: "real list" and f :: "real list \<Righ
 assumes "valid_tm I a f t"
 assumes "I all_subset J"
 assumes "a all_in I"
-shows "set_of (compute_bound_tm t I a) \<subseteq> set_of (compute_bound_tm t J a)"
+shows "set_of (compute_bound_tm I a t) \<subseteq> set_of (compute_bound_tm J a t)"
 apply(cases t, simp del: compute_bound_poly.simps)
 apply(rule set_of_add_inc_left)
 apply(rule compute_bound_poly_mono[OF _ assms(2,3)])
@@ -263,12 +263,12 @@ subsection \<open>Computing taylor models for basic, univariate functions\<close
 fun tm_const :: "float \<Rightarrow> taylor_model"
 where "tm_const c = TaylorModel (poly.C c) (Ivl 0 0)"
 
-fun tm_id :: "nat \<Rightarrow> float list \<Rightarrow> taylor_model"
-where "tm_id n a = TaylorModel (poly.CN (poly.C (a!n)) n (poly.C 1)) (Ivl 0 0)"
+fun tm_var :: "nat \<Rightarrow> float list \<Rightarrow> taylor_model"
+where "tm_var i a = TaylorModel (poly.CN (poly.C (a!i)) i (poly.C 1)) (Ivl 0 0)"
 
 fun tm_pi :: "nat \<Rightarrow> taylor_model"
 where "tm_pi prec = (
-  let pi_ivl=the (compute_bound prec Pi [])
+  let pi_ivl = the (compute_bound_fa prec Pi [])
   in TaylorModel (poly.C (mid pi_ivl)) (centered pi_ivl)
 )"
 
@@ -278,10 +278,10 @@ shows "valid_tm I a (interpret_floatarith (Num c)) (tm_const c)"
 using assms
 by simp
 
-lemma tm_id_valid:
+lemma tm_var_valid:
 assumes "n < length I"
 assumes "a all_in I"
-shows "valid_tm I a (interpret_floatarith (Var n)) (tm_id n a)"
+shows "valid_tm I a (interpret_floatarith (Var n)) (tm_var n a)"
 using assms by simp
 
 lemma tm_pi_valid:
@@ -291,14 +291,14 @@ proof-
   have "\<And>prec. real_of_float (lb_pi prec) \<le> real_of_float (ub_pi prec)"
     using iffD1[OF atLeastAtMost_iff, OF pi_boundaries]
     using order_trans by auto
-  then obtain ivl_pi where ivl_pi_def: "Some ivl_pi = compute_bound prec Pi []"
+  then obtain ivl_pi where ivl_pi_def: "Some ivl_pi = compute_bound_fa prec Pi []"
     by (simp add: approx.simps)
   show ?thesis
     apply(rule valid_tmI[OF _ _ assms])
-    apply(simp add: Let_def del: compute_bound.simps)
+    apply(simp add: Let_def del: compute_bound_fa.simps)
     apply(simp)
     unfolding ivl_pi_def[symmetric]
-    using compute_bound_correct[of "[]" "[]", OF _ ivl_pi_def, simplified]
+    using compute_bound_fa_correct[of "[]" "[]", OF _ ivl_pi_def, simplified]
     by (simp, simp add: minus_interval_def set_of_def)
 qed
 
@@ -420,28 +420,46 @@ shows "deriv_0 f 0 = f"
 by (cases "(f, 0::nat)" rule: deriv_0.cases, simp_all)
 
 
-subsubsection \<open>Automatic computation of taylor coefficients for univariate functions\<close>
+subsubsection \<open>Computing taylor models for arbitrary univariate expressions\<close> 
 
 (* The interval coefficients of the taylor polynomial,
    i.e. the real coefficients approximated by a float interval. *)
 fun tmf_c :: "nat \<Rightarrow> nat \<Rightarrow> float interval \<Rightarrow> floatarith \<Rightarrow> float interval option"
-where "tmf_c prec n i f = compute_bound prec (Mult (deriv_0 f n) (Inverse (Num (fact n)))) [i]"
+where "tmf_c prec n i f = compute_bound_fa prec (Mult (deriv_0 f n) (Inverse (Num (fact n)))) [i]"
 
 (* Make a list of the n coefficients. *) 
-fun tmf_cs' :: "nat \<Rightarrow> nat \<Rightarrow> float interval \<Rightarrow> float \<Rightarrow> floatarith \<Rightarrow> float interval option list"
+fun tmf_cs' :: "nat \<Rightarrow> nat \<Rightarrow> float interval \<Rightarrow> float interval \<Rightarrow> floatarith \<Rightarrow> float interval option list"
 where "tmf_cs' _ 0 I a f = []"
-    | "tmf_cs' prec (Suc n) I a f = (tmf_c prec n (interval_of a) f) # (tmf_cs' prec n I a f)"
+    | "tmf_cs' prec (Suc n) I a f = (tmf_c prec n a f) # (tmf_cs' prec n I a f)"
 
 (* Also add the n+1-th coefficient, representing the error contribution, and reorder the list. *)
 fun tmf_cs :: "nat \<Rightarrow> nat \<Rightarrow> float interval \<Rightarrow> float \<Rightarrow> floatarith \<Rightarrow> float interval list option"
 where "tmf_cs prec n I a f = those (rev (tmf_c prec n I f # (tmf_cs' prec n I a f)))"
+
+fun tm_floatarith' :: "float interval list \<Rightarrow> float poly \<times> float interval poly"
+where "tm_floatarith' [] = (poly.C 0, poly.C 0)"
+    | "tm_floatarith' (c # cs) = (
+         let (pf, pi) = tm_floatarith' cs
+         in (poly.CN (poly.C (mid c)) 0 pf, poly.CN (poly.C (centered c)) 0 pi)
+       )"
+
+(* Compute a taylor model from an arbitrary, univariate floatarith expression, if possible.
+   This is used to compute taylor models for elemental functions like sin, cos, exp, etc. *)
+fun tm_floatarith :: "nat \<Rightarrow> nat \<Rightarrow> float interval \<Rightarrow> float \<Rightarrow> floatarith \<Rightarrow> taylor_model option"
+where "tm_floatarith prec ord I a f = (
+  map_option (\<lambda>cs. 
+    let (pf, pi) = tm_floatarith' cs;
+        e = round_ivl prec (Ipoly [I - interval_of a] pi)
+    in TaylorModel pf e
+  ) (tmf_cs prec ord I a f)
+)"
 
 lemma tmf_c_correct:
 fixes A::"float interval" and I::"float interval" and f::floatarith and a::real
 assumes "a \<in> set_of A"
 assumes "Some I = tmf_c prec i A f"
 shows "interpret_floatarith (deriv_0 f i) [a] / fact i \<in> set_of I"
-using compute_bound_correct[OF _  assms(2)[unfolded tmf_c.simps], where i="[a]"] assms(1)
+using compute_bound_fa_correct[OF _  assms(2)[unfolded tmf_c.simps], where i="[a]"] assms(1)
 by (simp add: divide_real_def fact_real_float_equiv)
 
 lemma tmf_cs_length:
@@ -490,18 +508,6 @@ next
   finally show "Some (cs ! i) = tmf_c prec i (interval_of a) f" .
 qed
 
-
-subsubsection \<open>Computing taylor models for arbitrary univariate expressions\<close> 
-
-fun tm_floatarith' :: "float interval list \<Rightarrow> float poly \<times> float interval poly"
-where "tm_floatarith' [] = (poly.C 0, poly.C 0)"
-    | "tm_floatarith' (c # cs) = (\<lambda>(pf, pi). (poly.CN (poly.C (mid c)) 0 pf, poly.CN (poly.C (centered c)) 0 pi)) (tm_floatarith' cs)"
-
-(* Compute a taylor model from an arbitrary, univariate floatarith expression, if possible.
-   This is used to compute taylor models for elemental functions like sin, cos, exp, etc. *)
-fun tm_floatarith :: "nat \<Rightarrow> nat \<Rightarrow> float interval \<Rightarrow> float \<Rightarrow> floatarith \<Rightarrow> taylor_model option"
-where "tm_floatarith prec ord I a f = map_option (\<lambda>(pf, pi). TaylorModel pf (Ipoly [I - interval_of a] pi)) (map_option tm_floatarith' (tmf_cs prec ord I a f))"
-
 (* TODO: Clean this up! *)
 lemma tm_floatarith_valid:
 assumes "0 < ord"
@@ -510,24 +516,26 @@ assumes "\<And>x. x \<in> set_of I \<Longrightarrow> isDERIV 0 f [x]"
 assumes "Some t = tm_floatarith prec ord I a f"
 shows "valid_tm [I] [a] (interpret_floatarith f) t"
 proof-
-  from assms(4)[unfolded tm_floatarith.simps]
-  obtain pf pi where Some_pf_pi_def: "Some (pf, pi) = map_option tm_floatarith' (tmf_cs prec ord I a f)"
-    by (metis (no_types, lifting) map_option_eq_Some prod.collapse)
-  then have t_def: "t = TaylorModel pf (Ipoly [I - interval_of a] pi)"
+  obtain cs where cs_def: "Some cs = tmf_cs prec ord I a f"
+    using assms(4)[unfolded tm_floatarith.simps, symmetric]
+      by auto
+  from assms(4)[unfolded tm_floatarith.simps] 
+  obtain pf pi where pf_pi_def: "(pf, pi) = tm_floatarith' cs"
+    unfolding cs_def[symmetric]
+    using prod.collapse by blast
+  
+  have t_def: "t = TaylorModel pf (round_ivl prec (Ipoly [I - interval_of a] pi))"
     using assms(4)[unfolded tm_floatarith.simps]
-    by (metis old.prod.case option.sel option.simps(9))
-  from Some_pf_pi_def obtain cs where cs_def: "Some cs = tmf_cs prec ord I a f"
-    by (metis map_option_eq_Some)
-  have pfpi_def: "(pf, pi) = tm_floatarith' cs"
-    by (metis Some_pf_pi_def cs_def map_option_eq_Some option.sel)
+    unfolding cs_def[symmetric]
+    by (simp add: pf_pi_def[symmetric])
   
   show ?thesis
   proof(rule valid_tmI)
-    show "t = TaylorModel pf (Ipoly [I - interval_of a] pi)"
+    show "t = TaylorModel pf (round_ivl prec (Ipoly [I - interval_of a] pi))"
       by (simp add: t_def)
   next
     show "num_params pf \<le> length [I]"
-      using pfpi_def
+      using pf_pi_def
       apply(induction cs arbitrary: pf pi)
       apply(simp)
       proof-
@@ -546,12 +554,12 @@ proof-
     from hyp obtain x where xs_def: "xs = [x]" by (auto simp: length_Suc_conv)
     hence x_in_I: "x \<in> set_of I" using hyp by simp
     
-    show "interpret_floatarith f xs - Ipoly (list_op op- xs [a]) pf
+    have "interpret_floatarith f xs - Ipoly (list_op op- xs [a]) pf
          \<in> set_of (interval_map real_of_float (Ipoly [I - interval_of a] pi))"
     proof(cases "x = a")
       case True
       have pf_val_at_a: "Ipoly (list_op op- xs [a]) pf = mid (cs ! 0)"
-        using pfpi_def tmf_cs_length[OF cs_def]
+        using pf_pi_def tmf_cs_length[OF cs_def]
         apply(induction cs arbitrary: pf pi ord)
         apply(simp)
         proof-
@@ -575,7 +583,7 @@ proof-
           obtain c cs' where cs_decomp: "cs = c # cs'" 
             by (metis Suc_eq_plus1 list.size(3) neq_Nil_conv old.nat.distinct(2))
           obtain pi' where pi_decomp: "pi = poly.CN (c - interval_of (mid c))\<^sub>p 0 pi'"
-            using pfpi_def
+            using pf_pi_def
             by (simp add: cs_decomp case_prod_beta)
           show ?thesis
             apply(simp add: cs_decomp pi_decomp)
@@ -618,7 +626,7 @@ proof-
         apply(simp add: I_def set_of_def)
         by (meson less_eq_real_def order_trans)
       
-      from pfpi_def tmf_cs_length[OF cs_def]
+      from pf_pi_def tmf_cs_length[OF cs_def]
       have Ipoly_pf_eq: "Ipoly (list_op op- xs [a]) pf = (\<Sum>m<Suc ord. mid (cs!m) * (x - a) ^ m)"
         apply(induction cs arbitrary: ord pf pi)
         apply(simp add: xs_def)
@@ -690,7 +698,7 @@ proof-
             by simp
         qed
       also have "... \<subseteq> set_of (interval_map real_of_float (Ipoly [I - interval_of a] pi))"
-        using ci_def pfpi_def tmf_cs_length[OF cs_def]
+        using ci_def pf_pi_def tmf_cs_length[OF cs_def]
         proof(induction ord arbitrary: cs pi pf ci)
           case (0 cs pi pf)
           from 0(2) obtain c where cs_def: "cs = [c]"
@@ -730,6 +738,11 @@ proof-
         using taylor_expansion
         by (simp add: xs_def)
     qed
+    also have "... \<subseteq> set_of (round_ivl prec (Ipoly [I - interval_of a] pi))"
+      using real_of_float_round_ivl_correct by auto
+    finally show "interpret_floatarith f xs - Ipoly (list_op op- xs (map real_of_float [a])) (pf)
+                  \<in> set_of (round_ivl prec (Ipoly [I - interval_of a] pi))"
+      .
   next
     show "[a] all_in [I]"
       using \<open>a \<in> set_of I\<close>
@@ -745,89 +758,104 @@ fun tm_norm_poly :: "taylor_model \<Rightarrow> taylor_model"
 where "tm_norm_poly (TaylorModel p e) = TaylorModel (polynate p) e"
 
 (* Reduces the degree of a taylor model's polynomial to n and keeps it valid by increasing the error bound. *)
-fun tm_lower_order tm_lower_order_of_normed :: "nat \<Rightarrow> taylor_model \<Rightarrow> float interval list \<Rightarrow> float list \<Rightarrow> taylor_model"
-where "tm_lower_order ord t I a = tm_lower_order_of_normed ord (tm_norm_poly t) I a"
-   |  "tm_lower_order_of_normed ord (TaylorModel p e) I a = (
+fun tm_lower_order tm_lower_order_of_normed :: "nat \<Rightarrow> float interval list \<Rightarrow> float list \<Rightarrow> taylor_model \<Rightarrow> taylor_model"
+where "tm_lower_order ord I a t = tm_lower_order_of_normed ord I a (tm_norm_poly t)"
+   |  "tm_lower_order_of_normed ord I a (TaylorModel p e) = (
          let (l, r) = split_by_degree ord p
          in TaylorModel l (e + compute_bound_poly r I a)
        )"
 
 (* We also round our float coefficients. *)
-fun tm_round_floats tm_round_floats_of_normed :: "nat \<Rightarrow> taylor_model \<Rightarrow> float interval list \<Rightarrow> float list \<Rightarrow> taylor_model"
-where "tm_round_floats prec t I a = tm_round_floats_of_normed prec (tm_norm_poly t) I a"
-    | "tm_round_floats_of_normed prec (TaylorModel p e) I a = (
+fun tm_round_floats tm_round_floats_of_normed :: "nat \<Rightarrow> float interval list \<Rightarrow> float list \<Rightarrow> taylor_model \<Rightarrow> taylor_model"
+where "tm_round_floats prec I a t = tm_round_floats_of_normed prec I a (tm_norm_poly t)"
+    | "tm_round_floats_of_normed prec I a (TaylorModel p e) = (
          let (l, r) = split_by_prec prec p
          in TaylorModel l (round_ivl prec (e + compute_bound_poly r I a))
        )"
 
 (* Order lowering and rounding on tayor models, also converts the polynomial into horner form. *)
-fun tm_norm tm_norm' :: "nat \<Rightarrow> nat \<Rightarrow> taylor_model \<Rightarrow> float interval list \<Rightarrow> float list \<Rightarrow> taylor_model"
-where "tm_norm prec ord t I a = tm_norm' prec ord (tm_norm_poly t) I a"
-    | "tm_norm' prec ord t I a = tm_round_floats_of_normed prec (tm_lower_order_of_normed ord t I a) I a" 
+fun tm_norm tm_norm' :: "nat \<Rightarrow> nat \<Rightarrow> float interval list \<Rightarrow> float list \<Rightarrow> taylor_model \<Rightarrow> taylor_model"
+where "tm_norm prec ord I a t = tm_norm' prec ord I a (tm_norm_poly t)"
+    | "tm_norm' prec ord I a t = tm_round_floats_of_normed prec I a (tm_lower_order_of_normed ord I a t)" 
 
 fun tm_neg :: "taylor_model \<Rightarrow> taylor_model"
-where "tm_neg (TaylorModel p i) = TaylorModel (~\<^sub>p p) (-i)"
+where "tm_neg (TaylorModel p e) = TaylorModel (~\<^sub>p p) (-e)"
 
 fun tm_add :: "taylor_model \<Rightarrow> taylor_model \<Rightarrow> taylor_model"
-where "tm_add (TaylorModel p1 i1) (TaylorModel p2 i2) = TaylorModel (p1 +\<^sub>p p2) (i1+i2)"
+where "tm_add (TaylorModel p1 e1) (TaylorModel p2 e2) = TaylorModel (p1 +\<^sub>p p2) (e1 + e2)"
 
 fun tm_sub :: "taylor_model \<Rightarrow> taylor_model \<Rightarrow> taylor_model"
 where "tm_sub t1 t2 = tm_add t1 (tm_neg t2)"
 
 (* Note: This increases the degree of the polynomial. tm_lower_order can be used to reduce it again. *)
-fun tm_mul :: "nat \<Rightarrow> nat \<Rightarrow> taylor_model \<Rightarrow> taylor_model \<Rightarrow> float interval list \<Rightarrow> float list \<Rightarrow> taylor_model"
-where "tm_mul prec ord (TaylorModel p1 i1) (TaylorModel p2 i2) I a = (
-  let d1=compute_bound_poly p1 I a;
-      d2=compute_bound_poly p2 I a
-  in tm_norm' prec ord (TaylorModel (p1 *\<^sub>p p2) (i1*d2 + d1*i2 + i1*i2))) I a"
+fun tm_mul :: "nat \<Rightarrow> nat \<Rightarrow> float interval list \<Rightarrow> float list \<Rightarrow> taylor_model \<Rightarrow> taylor_model \<Rightarrow> taylor_model"
+where "tm_mul prec ord I a (TaylorModel p1 e1) (TaylorModel p2 e2) = (
+         let d1 = compute_bound_poly p1 I a;
+             d2 = compute_bound_poly p2 I a;
+             p = p1 *\<^sub>p p2;
+             e = e1*d2 + d1*e2 + e1*e2
+         in tm_norm' prec ord I a (TaylorModel p e)
+       )"
   
-fun tm_pow :: "nat \<Rightarrow> nat \<Rightarrow> taylor_model \<Rightarrow> nat \<Rightarrow> float interval list \<Rightarrow> float list \<Rightarrow> taylor_model"
-where "tm_pow prec ord t 0 I a = tm_const 1"
-    | "tm_pow prec ord t (Suc n) I a = tm_mul prec ord t (tm_pow prec ord t n I a) I a"
+fun tm_pow :: "nat \<Rightarrow> nat \<Rightarrow> float interval list \<Rightarrow> float list \<Rightarrow> taylor_model \<Rightarrow> nat \<Rightarrow> taylor_model"
+where "tm_pow prec ord I a t 0 = tm_const 1"
+    | "tm_pow prec ord I a t (Suc n) = tm_mul prec ord I a t (tm_pow prec ord I a t n)"
 
 (* Evaluates a float polynomial, using a taylor model as the parameter. This is used to compose taylor models. *)
-fun eval_poly_at_tm :: "nat \<Rightarrow> nat \<Rightarrow> float poly \<Rightarrow> taylor_model \<Rightarrow> float interval list \<Rightarrow> float list \<Rightarrow> taylor_model"
-where "eval_poly_at_tm prec ord (poly.C c) t I a = tm_const c"
-    | "eval_poly_at_tm prec ord (poly.Bound n) t I a = t"
-    | "eval_poly_at_tm prec ord (poly.Add p1 p2) t I a = tm_add (eval_poly_at_tm prec ord p1 t I a) (eval_poly_at_tm prec ord p2 t I a)"
-    | "eval_poly_at_tm prec ord (poly.Sub p1 p2) t I a = tm_sub (eval_poly_at_tm prec ord p1 t I a) (eval_poly_at_tm prec ord p2 t I a)"
-    | "eval_poly_at_tm prec ord (poly.Mul p1 p2) t I a = tm_mul  prec ord(eval_poly_at_tm prec ord p1 t I a) (eval_poly_at_tm prec ord p2 t I a) I a"
-    | "eval_poly_at_tm prec ord (poly.Neg p) t I a = tm_neg (eval_poly_at_tm prec ord p t I a)"
-    | "eval_poly_at_tm prec ord (poly.Pw p n) t I a = tm_pow prec ord (eval_poly_at_tm prec ord p t I a) n I a"
-    | "eval_poly_at_tm prec ord (poly.CN c n p) t I a = tm_add (eval_poly_at_tm prec ord c t I a) (tm_mul prec ord t (eval_poly_at_tm prec ord p t I a) I a)"
+fun eval_poly_at_tm :: "nat \<Rightarrow> nat \<Rightarrow> float interval list \<Rightarrow> float list \<Rightarrow> float poly \<Rightarrow> taylor_model \<Rightarrow> taylor_model"
+where "eval_poly_at_tm prec ord I a (poly.C c) t = tm_const c"
+    | "eval_poly_at_tm prec ord I a (poly.Bound n) t = t"
+    | "eval_poly_at_tm prec ord I a (poly.Add p1 p2) t
+         = tm_add (eval_poly_at_tm prec ord I a p1 t)
+                  (eval_poly_at_tm prec ord I a p2 t)"
+    | "eval_poly_at_tm prec ord I a (poly.Sub p1 p2) t
+         = tm_sub (eval_poly_at_tm prec ord I a p1 t)
+                  (eval_poly_at_tm prec ord I a p2 t)"
+    | "eval_poly_at_tm prec ord I a (poly.Mul p1 p2) t
+         = tm_mul prec ord I a (eval_poly_at_tm prec ord I a  p1 t)
+                               (eval_poly_at_tm prec ord I a p2 t)"
+    | "eval_poly_at_tm prec ord I a (poly.Neg p) t
+         = tm_neg (eval_poly_at_tm prec ord I a p t)"
+    | "eval_poly_at_tm prec ord I a (poly.Pw p n) t
+         = tm_pow prec ord I a (eval_poly_at_tm prec ord I a p t) n"
+    | "eval_poly_at_tm prec ord I a (poly.CN c n p) t = (
+         let pt = eval_poly_at_tm prec ord I a p t;
+             t_mul_pt = tm_mul prec ord I a t pt 
+         in tm_add (eval_poly_at_tm prec ord I a c t) t_mul_pt
+       )"
 
-
-fun tm_inc_error :: "nat \<Rightarrow> taylor_model \<Rightarrow> float interval \<Rightarrow> taylor_model"
-where "tm_inc_error prec (TaylorModel p e) i = TaylorModel p (round_ivl prec (e+i))"
+fun tm_inc_err :: "float interval \<Rightarrow> taylor_model \<Rightarrow> taylor_model"
+where "tm_inc_err i (TaylorModel p e) = TaylorModel p (e + i)"
     
-fun tm_comp :: "nat \<Rightarrow> nat \<Rightarrow> taylor_model \<Rightarrow> taylor_model \<Rightarrow> float interval list \<Rightarrow> float list \<Rightarrow> float \<Rightarrow> taylor_model"
-where "tm_comp prec ord (TaylorModel p e) t I a ta = (
-         let t_minus_ta=tm_sub t (tm_const ta)
-         in tm_inc_error prec (eval_poly_at_tm prec ord p t_minus_ta I a) e
+fun tm_comp :: "nat \<Rightarrow> nat \<Rightarrow> float interval list \<Rightarrow> float list \<Rightarrow> float \<Rightarrow> taylor_model \<Rightarrow> taylor_model \<Rightarrow> taylor_model"
+where "tm_comp prec ord I a ta (TaylorModel p e) t = (
+         let t_sub_ta = tm_sub t (tm_const ta);
+             pt = eval_poly_at_tm prec ord I a p t_sub_ta
+         in tm_inc_err e pt
        )"
 
 (* tm_abs, tm_min and tm_max are implemented extremely naively, because I don't expect them to be very useful.
    But the implementation is fairly modular, i.e. tm_{abs,min,max} all can easily be swapped out,
    as long as the corresponding correctness lemmas tm_{abs,min,max}_valid are updated as well. *)
-fun tm_abs :: "taylor_model \<Rightarrow> float interval list \<Rightarrow> float list \<Rightarrow> taylor_model"
-where "tm_abs t I a = (
-  let bound = compute_bound_tm t I a; abs_bound=Ivl (0::float) (max (abs (lower bound)) (abs (upper bound)))
+fun tm_abs :: "float interval list \<Rightarrow> float list \<Rightarrow> taylor_model \<Rightarrow> taylor_model"
+where "tm_abs I a t = (
+  let bound = compute_bound_tm I a t; abs_bound=Ivl (0::float) (max (abs (lower bound)) (abs (upper bound)))
   in TaylorModel (poly.C (mid abs_bound)) (centered abs_bound))"
 
-fun tm_and :: "taylor_model \<Rightarrow> taylor_model \<Rightarrow> float interval list \<Rightarrow> float list \<Rightarrow> taylor_model"
-where "tm_and t1 t2 I a = (
-  let b1 = compute_bound_tm t1 I a; b2 = compute_bound_tm t2 I a;
+fun tm_and :: "float interval list \<Rightarrow> float list \<Rightarrow> taylor_model \<Rightarrow> taylor_model \<Rightarrow> taylor_model"
+where "tm_and I a t1 t2 = (
+  let b1 = compute_bound_tm I a t1; b2 = compute_bound_tm I a t2;
       b_combined = interval_union b1 b2
   in TaylorModel (poly.C (mid b_combined)) (centered b_combined))"
   
-fun tm_min :: "taylor_model \<Rightarrow> taylor_model \<Rightarrow> float interval list \<Rightarrow> float list \<Rightarrow> taylor_model"
-where "tm_min t1 t2 I a = tm_and t1 t2 I a"
+fun tm_min :: "float interval list \<Rightarrow> float list \<Rightarrow> taylor_model \<Rightarrow> taylor_model \<Rightarrow> taylor_model"
+where "tm_min I a t1 t2 = tm_and I a t1 t2"
   
-fun tm_max :: "taylor_model \<Rightarrow> taylor_model \<Rightarrow> float interval list \<Rightarrow> float list \<Rightarrow> taylor_model"
-where "tm_max t1 t2 I a = tm_and t1 t2 I a"
+fun tm_max :: "float interval list \<Rightarrow> float list \<Rightarrow> taylor_model \<Rightarrow> taylor_model \<Rightarrow> taylor_model"
+where "tm_max I a t1 t2 = tm_and I a t1 t2"
 
 
-(* Validity of is preserved under taylor model arithmetic. *)
+(* Validity of is preserved by our operations on taylor models. *)
 lemma tm_norm_poly_valid:
 assumes "valid_tm I a f t"
 shows "valid_tm I a f (tm_norm_poly t)"
@@ -839,7 +867,7 @@ by blast
 
 lemma tm_lower_order_of_normed_valid:
 assumes "valid_tm I a f t"
-shows "valid_tm I a f (tm_lower_order_of_normed ord t I a)"
+shows "valid_tm I a f (tm_lower_order_of_normed ord I a t)"
 proof-
   obtain p e where t_decomp: "t = TaylorModel p e"
     by (cases t) simp
@@ -848,7 +876,7 @@ proof-
   
   show ?thesis
   proof(rule valid_tmI)
-    show "tm_lower_order_of_normed ord t I a = TaylorModel pl (e + compute_bound_poly pr I a)"
+    show "tm_lower_order_of_normed ord I a t = TaylorModel pl (e + compute_bound_poly pr I a)"
     by (simp add: t_decomp p_split)
   next
     show "num_params pl \<le> length I"
@@ -882,13 +910,13 @@ qed
 
 lemma tm_lower_order_valid:
 assumes "valid_tm I a f t"
-shows "valid_tm I a f (tm_lower_order ord t I a)"
+shows "valid_tm I a f (tm_lower_order ord I a t)"
 using assms tm_lower_order_of_normed_valid tm_norm_poly_valid
 by simp
 
 lemma tm_round_floats_of_normed_valid:
 assumes "valid_tm I a f t"
-shows "valid_tm I a f (tm_round_floats_of_normed prec t I a)"
+shows "valid_tm I a f (tm_round_floats_of_normed prec I a t)"
 proof-
   obtain p e where t_decomp: "t = TaylorModel p e"
     by (cases t) simp
@@ -897,7 +925,7 @@ proof-
   
   show ?thesis
   proof(rule valid_tmI)
-    show "tm_round_floats_of_normed prec t I a = TaylorModel pl (round_ivl prec (e + compute_bound_poly pr I a))"
+    show "tm_round_floats_of_normed prec I a t = TaylorModel pl (round_ivl prec (e + compute_bound_poly pr I a))"
     by (simp add: t_decomp p_prec)
   next
     show "num_params pl \<le> length I"
@@ -933,19 +961,19 @@ qed
 
 lemma tm_round_floats_valid:
 assumes "valid_tm I a f t"
-shows "valid_tm I a f (tm_round_floats prec t I a)"
+shows "valid_tm I a f (tm_round_floats prec I a t)"
 using assms tm_round_floats_of_normed_valid tm_norm_poly_valid
 by simp
 
 lemma tm_norm'_valid:
 assumes "valid_tm I a f t" 
-shows "valid_tm I a f (tm_norm' prec ord t I a)"
+shows "valid_tm I a f (tm_norm' prec ord I a t)"
 using tm_round_floats_of_normed_valid[OF tm_lower_order_of_normed_valid[OF assms]]
 by simp
 
 lemma tm_norm_valid:
 assumes "valid_tm I a f t"
-shows "valid_tm I a f (tm_norm prec ord t I a)"
+shows "valid_tm I a f (tm_norm prec ord I a t)"
 using assms tm_norm'_valid tm_norm_poly_valid
 by simp
 
@@ -1027,7 +1055,7 @@ by simp
 lemma tm_mul_valid:
 assumes "valid_tm I a f t1"
 assumes "valid_tm I a g t2"
-shows "valid_tm I a (f * g) (tm_mul prec ord t1 t2 I a)"
+shows "valid_tm I a (f * g) (tm_mul prec ord I a t1 t2)"
 proof-
   from valid_tmD[OF assms(1)]
   obtain p1 i1 where t1_def:
@@ -1044,7 +1072,7 @@ proof-
     "\<And>x::real list. x all_in I \<Longrightarrow> g x - Ipoly (list_op op- x (a::real list)) p2 \<in> set_of i2"
       by blast
       
-  show "valid_tm I a (f * g) (tm_mul prec ord t1 t2 I a)"
+  show "valid_tm I a (f * g) (tm_mul prec ord I a t1 t2)"
     unfolding t1_def t2_def tm_mul.simps Let_def
     apply(rule tm_norm'_valid)
     apply(rule valid_tmI[OF _ _ \<open>a all_in I\<close>])
@@ -1090,7 +1118,7 @@ qed
 
 lemma tm_pow_valid:
 assumes "valid_tm I a f t"
-shows "valid_tm I a (f ^ n) (tm_pow prec ord t n I a)"
+shows "valid_tm I a (f ^ n) (tm_pow prec ord I a t n)"
 apply(induction n)
 apply(simp)
 using all_in_def assms
@@ -1101,7 +1129,7 @@ by (simp add: func_times)
 lemma eval_poly_at_tm_valid:
 assumes "num_params p \<le> 1"
 assumes tg_def: "valid_tm I a g tg"
-shows "valid_tm I a ((\<lambda>x. Ipoly ([x]) p) o g) (eval_poly_at_tm prec ord p tg I a)"
+shows "valid_tm I a ((\<lambda>x. Ipoly ([x]) p) o g) (eval_poly_at_tm prec ord I a p tg)"
 using assms(1)
 proof(induction p)
   case (C c) thus ?case
@@ -1135,7 +1163,7 @@ lemma tm_comp_valid:
 assumes gI_def: "\<And>x. x all_in I \<Longrightarrow> g x \<in> set_of gI"
 assumes tf_def: "valid_tm [gI] [ga] (\<lambda>x. f (x ! 0)) tf"
 assumes tg_def: "valid_tm I a g tg"
-shows "valid_tm I a (f o g) (tm_comp prec ord tf tg I a ga)"
+shows "valid_tm I a (f o g) (tm_comp prec ord I a ga tf tg)"
 proof-
   obtain pf ef where tf_decomp: "tf = TaylorModel pf ef" using taylor_model.exhaust by auto
   obtain pg eg where tg_decomp: "tg = TaylorModel pg eg" using taylor_model.exhaust by auto
@@ -1160,14 +1188,14 @@ proof-
     "\<And>x::real list. x all_in I \<Longrightarrow> g x - Ipoly (list_op op- x (a::real list)) pg \<in> set_of eg"
       by simp_all
       
-  obtain p' e' where p'e'_def: "TaylorModel p' e' = eval_poly_at_tm prec ord pf (tm_sub tg (tm_const ga)) I a"
+  obtain p' e' where p'e'_def: "TaylorModel p' e' = eval_poly_at_tm prec ord I a pf (tm_sub tg (tm_const ga))"
     using taylor_model.exhaust by smt
   
   have "valid_tm I a (\<lambda>x. g x - ga) (tm_sub tg (tm_const ga))"
     using tm_sub_valid[OF tg_def tm_const_valid[OF \<open>a all_in I\<close>, of ga]]
     by auto
   from eval_poly_at_tm_valid[OF tf_valid(1) this]
-  have "valid_tm I a ((\<lambda>x. Ipoly ([x - ga]) pf) o g) (eval_poly_at_tm prec ord pf (tm_sub tg (tm_const ga)) I a)"
+  have "valid_tm I a ((\<lambda>x. Ipoly ([x - ga]) pf) o g) (eval_poly_at_tm prec ord I a pf (tm_sub tg (tm_const ga)))"
     by (simp add: comp_def)
   from valid_tmD'[OF this p'e'_def[symmetric]]
   have eval_poly_at_tm_valid:
@@ -1179,7 +1207,7 @@ proof-
       by auto
   show ?thesis
     proof(rule valid_tmI)
-      show "tm_comp prec ord tf tg I a ga = TaylorModel p' (round_ivl prec (e'+ef))"
+      show "tm_comp prec ord I a ga tf tg = TaylorModel p' (e'+ef)"
         using p'e'_def[symmetric]
         by (simp add: tf_decomp)
     next
@@ -1193,24 +1221,20 @@ proof-
       have "Ipoly [g x - ga] pf - Ipoly (list_op op- x (a::real list)) p' \<in> set_of e'"
         using eval_poly_at_tm_valid(2)[OF \<open>x all_in I\<close>]
         by simp
-      hence "(f \<circ> g) x - Ipoly (list_op op- x (a::real list)) p' \<in> set_of (e' + ef)"
+      thus "(f \<circ> g) x - Ipoly (list_op op- x (a::real list)) p' \<in> set_of (e' + ef)"
         using set_of_add_mono tf_g_valid[OF \<open>x all_in I\<close>]
         by force
-      also have "... \<subseteq> set_of (round_ivl prec (e' + ef) :: real interval)"
-        by (rule real_of_float_round_ivl_correct)
-      finally show "(f \<circ> g) x - Ipoly (list_op op- x a) p' \<in> set_of (round_ivl prec (e' + ef) :: real interval)"
-        .
     qed
 qed
 
 lemma tm_abs_valid:
 assumes "valid_tm I a f t"
-shows "valid_tm I a (abs o f) (tm_abs t I a)"
+shows "valid_tm I a (abs o f) (tm_abs I a t)"
 proof-
   obtain p e where t_def[simp]: "t = TaylorModel p e" using taylor_model.exhaust by auto
-  def bound\<equiv>"compute_bound_tm (TaylorModel p e) I a"
+  def bound\<equiv>"compute_bound_tm I a (TaylorModel p e)"
   def abs_bound\<equiv>"Ivl 0 (max \<bar>lower bound\<bar> \<bar>upper bound\<bar>)"
-  have tm_abs_decomp: "tm_abs t I a =  TaylorModel (poly.C (mid abs_bound)) (centered abs_bound)"
+  have tm_abs_decomp: "tm_abs I a t =  TaylorModel (poly.C (mid abs_bound)) (centered abs_bound)"
     by (simp add: bound_def abs_bound_def Let_def)
   show ?thesis
     apply(rule valid_tmI[OF tm_abs_decomp])
@@ -1228,13 +1252,14 @@ qed
 
 lemma tm_and_valid_left:
 assumes "valid_tm I a f t1"
-shows "valid_tm I a f (tm_and t1 t2 I a)"
+shows "valid_tm I a f (tm_and I a t1 t2)"
 proof-
-  def b1\<equiv>"compute_bound_tm t1 I a"
-  def b2\<equiv>"compute_bound_tm t2 I a"
+  def b1\<equiv>"compute_bound_tm I a t1"
+  def b2\<equiv>"compute_bound_tm I a t2"
   def b_combined\<equiv>"Ivl (min (lower b1) (lower b2)) (max (upper b1) (upper b2))"
 
-  obtain p e where tm_and_decomp: "tm_and t1 t2 I a = TaylorModel p e" using taylor_model.exhaust by auto
+  obtain p e where tm_and_decomp: "tm_and I a t1 t2 = TaylorModel p e"
+    using taylor_model.exhaust by auto
   then have p_def: "p = (mid b_combined)\<^sub>p"
         and e_def: "e = centered b_combined"
     by (auto simp: Let_def b1_def b2_def b_combined_def interval_union_def)
@@ -1252,16 +1277,16 @@ qed
 
 lemma tm_and_valid_right:
 assumes "valid_tm I a g t2"
-shows "valid_tm I a g (tm_and t1 t2 I a)"
+shows "valid_tm I a g (tm_and I a t1 t2)"
 using tm_and_valid_left[OF assms]
 by (simp add: interval_union_commute)
 
 lemma tm_min_valid:
 assumes "valid_tm I a f t1"
 assumes "valid_tm I a g t2"
-shows "valid_tm I a (\<lambda>x. min (f x) (g x)) (tm_min t1 t2 I a)"
+shows "valid_tm I a (\<lambda>x. min (f x) (g x)) (tm_min I a t1 t2)"
 proof-
-  obtain p e where tm_and_decomp: "tm_and t1 t2 I a = TaylorModel p e"
+  obtain p e where tm_and_decomp: "tm_and I a t1 t2 = TaylorModel p e"
     using taylor_model.exhaust by auto
   
   note a = valid_tmD'[OF tm_and_valid_left[OF assms(1)] tm_and_decomp]
@@ -1280,9 +1305,9 @@ qed
 lemma tm_max_valid:
 assumes "valid_tm I a f t1"
 assumes "valid_tm I a g t2"
-shows "valid_tm I a (\<lambda>x. max (f x) (g x)) (tm_max t1 t2 I a)"
+shows "valid_tm I a (\<lambda>x. max (f x) (g x)) (tm_max I a t1 t2)"
 proof-
-  obtain p e where tm_and_decomp: "tm_and t1 t2 I a = TaylorModel p e"
+  obtain p e where tm_and_decomp: "tm_and I a t1 t2 = TaylorModel p e"
     using taylor_model.exhaust by auto
   
   note a = valid_tmD'[OF tm_and_valid_left[OF assms(1)] tm_and_decomp]
@@ -1303,49 +1328,58 @@ subsection \<open>Computing taylor models for multivariate expressions\<close>
 
 (* Compute taylor models for expressions of the form "f (g x)", where f is an elementary function like exp or cos,
    by composing taylor models for f and g. For our correctness proof, we need to make it explicit that the range
-   of g on I is inside the domain of f, by introducing the f_valid_on predicate. *)
+   of g on I is inside the domain of f, by introducing the f_exists_on predicate. *)
 fun compute_tm_by_comp :: "nat \<Rightarrow> nat \<Rightarrow> float interval list \<Rightarrow> float list \<Rightarrow> floatarith \<Rightarrow> taylor_model option \<Rightarrow> (float interval \<Rightarrow> bool) \<Rightarrow> taylor_model option"
-where "compute_tm_by_comp prec ord I a f g f_valid_on = (
+where "compute_tm_by_comp prec ord I a f g f_exists_on = (
          case g
          of Some tg \<Rightarrow> (
-           let gI = (compute_bound_tm tg I a); ga = mid (compute_bound_tm tg a a)
-           in (
-             if f_valid_on gI
-             then (case tm_floatarith prec ord gI ga f
-                   of Some tf \<Rightarrow> Some (tm_comp prec ord tf tg I a ga)
-                   | _ \<Rightarrow> None)
-             else None))
-         | _ \<Rightarrow> None)"
+           let gI = compute_bound_tm I a tg;
+               ga = mid (compute_bound_tm a a tg)
+           in if f_exists_on gI
+              then map_option (\<lambda>tf. tm_comp prec ord I a ga tf tg ) (tm_floatarith prec ord gI ga f)
+              else None)
+         | _ \<Rightarrow> None
+       )"
 
 (* Compute taylor models of degree n from floatarith expressions. *)
 fun compute_tm :: "nat \<Rightarrow> nat \<Rightarrow> float interval list \<Rightarrow> float list \<Rightarrow> floatarith \<Rightarrow> taylor_model option"
 where "compute_tm _ _ I _ (Num c) = Some (tm_const c)"
-    | "compute_tm _ _ I a (Var n) = Some (tm_id n a)"
+    | "compute_tm _ _ I a (Var n) = Some (tm_var n a)"
     | "compute_tm prec ord I a (Add l r) = (
          case (compute_tm prec ord I a l, compute_tm prec ord I a r) 
          of (Some t1, Some t2) \<Rightarrow> Some (tm_add t1 t2)
           | _ \<Rightarrow> None)"
-    | "compute_tm prec ord I a (Minus f) = map_option tm_neg (compute_tm prec ord I a f)"
+    | "compute_tm prec ord I a (Minus f)
+         = map_option tm_neg (compute_tm prec ord I a f)"
     | "compute_tm prec ord I a (Mult l r) = (
          case (compute_tm prec ord I a l, compute_tm prec ord I a r) 
-         of (Some t1, Some t2) \<Rightarrow> Some (tm_mul prec ord t1 t2 I a)
+         of (Some t1, Some t2) \<Rightarrow> Some (tm_mul prec ord I a t1 t2)
           | _ \<Rightarrow> None)"     
-    | "compute_tm prec ord I a (Power f k) = map_option (\<lambda>t. tm_pow prec ord t k I a) (compute_tm prec ord I a f)"
-    | "compute_tm prec ord I a (Inverse f) = compute_tm_by_comp prec ord I a (Inverse (Var 0)) (compute_tm prec ord I a f) (\<lambda>x. 0 < lower x \<or> upper x < 0)"
-    | "compute_tm prec ord I a (Cos f) = compute_tm_by_comp prec ord I a (Cos (Var 0)) (compute_tm prec ord I a f) (\<lambda>x. True)"
-    | "compute_tm prec ord I a (Arctan f) = compute_tm_by_comp prec ord I a (Arctan (Var 0)) (compute_tm prec ord I a f) (\<lambda>x. True)"
-    | "compute_tm prec ord I a (Exp f) = compute_tm_by_comp prec ord I a (Exp (Var 0)) (compute_tm prec ord I a f) (\<lambda>x. True)"
-    | "compute_tm prec ord I a (Ln f) = compute_tm_by_comp prec ord I a (Ln (Var 0)) (compute_tm prec ord I a f) (\<lambda>x. 0 < lower x)"
-    | "compute_tm prec ord I a (Sqrt f) = compute_tm_by_comp prec ord I a (Sqrt (Var 0)) (compute_tm prec ord I a f) (\<lambda>x. 0 < lower x)"
+    | "compute_tm prec ord I a (Power f k)
+         = map_option (\<lambda>t. tm_pow prec ord I a t k)
+                      (compute_tm prec ord I a f)"
+    | "compute_tm prec ord I a (Inverse f)
+         = compute_tm_by_comp prec ord I a (Inverse (Var 0)) (compute_tm prec ord I a f) (\<lambda>x. 0 < lower x \<or> upper x < 0)"
+    | "compute_tm prec ord I a (Cos f)
+         = compute_tm_by_comp prec ord I a (Cos (Var 0)) (compute_tm prec ord I a f) (\<lambda>x. True)"
+    | "compute_tm prec ord I a (Arctan f)
+         = compute_tm_by_comp prec ord I a (Arctan (Var 0)) (compute_tm prec ord I a f) (\<lambda>x. True)"
+    | "compute_tm prec ord I a (Exp f)
+         = compute_tm_by_comp prec ord I a (Exp (Var 0)) (compute_tm prec ord I a f) (\<lambda>x. True)"
+    | "compute_tm prec ord I a (Ln f)
+         = compute_tm_by_comp prec ord I a (Ln (Var 0)) (compute_tm prec ord I a f) (\<lambda>x. 0 < lower x)"
+    | "compute_tm prec ord I a (Sqrt f)
+         = compute_tm_by_comp prec ord I a (Sqrt (Var 0)) (compute_tm prec ord I a f) (\<lambda>x. 0 < lower x)"
     | "compute_tm prec ord I a Pi = Some (tm_pi prec)"
-    | "compute_tm prec ord I a (Abs f) = map_option (\<lambda>t. tm_abs t I a) (compute_tm prec ord I a f)"
+    | "compute_tm prec ord I a (Abs f)
+         = map_option (tm_abs I a) (compute_tm prec ord I a f)"
     | "compute_tm prec ord I a (Min l r) = (
          case (compute_tm prec ord I a l, compute_tm prec ord I a r) 
-         of (Some t1, Some t2) \<Rightarrow> Some (tm_min t1 t2 I a)
+         of (Some t1, Some t2) \<Rightarrow> Some (tm_min I a t1 t2)
           | _ \<Rightarrow> None)"
     | "compute_tm prec ord I a (Max l r) = (
          case (compute_tm prec ord I a l, compute_tm prec ord I a r) 
-         of (Some t1, Some t2) \<Rightarrow> Some (tm_max t1 t2 I a)
+         of (Some t1, Some t2) \<Rightarrow> Some (tm_max I a t1 t2)
           | _ \<Rightarrow> None)"
 
 lemma compute_tm_by_comp_valid:
@@ -1353,17 +1387,17 @@ assumes "0 < ord"
 assumes "num_vars f \<le> 1"
 assumes tx_valid: "valid_tm I a (interpret_floatarith g) tg"
 assumes t_def: "Some t = compute_tm_by_comp prec ord I a f (Some tg) c"
-assumes f_deriv: "\<And>x. x \<in> set_of (interval_map real_of_float (compute_bound_tm tg I a)) \<Longrightarrow> c (compute_bound_tm tg I a) \<Longrightarrow> isDERIV 0 f [x]"
+assumes f_deriv: "\<And>x. x \<in> set_of (interval_map real_of_float (compute_bound_tm I a tg)) \<Longrightarrow> c (compute_bound_tm I a tg) \<Longrightarrow> isDERIV 0 f [x]"
 shows "valid_tm I a ((\<lambda>x. interpret_floatarith f [x]) o interpret_floatarith g) t"
 proof-
   from t_def[simplified, simplified Let_def]
   obtain tf
-  where t1_def: "Some tf = tm_floatarith prec ord (compute_bound_tm tg I a) (mid (compute_bound_tm tg (map interval_of a) a)) f"
-  and t_decomp: "t = tm_comp prec ord tf tg I a (mid (compute_bound_tm tg (map interval_of a) a))"
-  and c_true:   "c (compute_bound_tm tg I a)"
+  where t1_def: "Some tf = tm_floatarith prec ord (compute_bound_tm I a tg) (mid (compute_bound_tm (map interval_of a) a tg)) f"
+  and t_decomp: "t = tm_comp prec ord I a (mid (compute_bound_tm (map interval_of a) a tg)) tf tg "
+  and c_true:   "c (compute_bound_tm I a tg)"
     unfolding Let_def
-    by (metis (no_types, lifting) option.case_eq_if option.collapse option.distinct(1) option.sel)
-  have a1: "mid (compute_bound_tm tg (map interval_of a) a) \<in> set_of (compute_bound_tm tg I a)"
+    by (smt option.collapse option.distinct(1) option.map_sel option.sel option.simps(8))
+  have a1: "mid (compute_bound_tm (map interval_of a) a tg) \<in> set_of (compute_bound_tm I a tg)"
     apply(rule rev_subsetD[OF mid_in_interval compute_bound_tm_mono[OF valid_tm_subset[OF _ _ tx_valid]]])
     using tx_valid
     by (auto simp add: set_of_def)
@@ -1429,7 +1463,7 @@ next
     by (metis (no_types, lifting) Mult(4) compute_tm.simps(5) option.case_eq_if option.collapse prod.case)
   obtain t2 where t2_def: "Some t2 = compute_tm prec ord I a r"
     by (smt Mult(4) compute_tm.simps(5) option.case_eq_if option.collapse prod.case)
-  have t_def: "t = tm_mul prec ord t1 t2 I a"
+  have t_def: "t = tm_mul prec ord I a t1 t2"
     using Mult(4) t1_def t2_def
     by (metis compute_tm.simps(5) option.case(2) option.inject prod.case)
   
@@ -1444,7 +1478,7 @@ next
   from Power(3)
   obtain tm_f where tm_f_def: "Some tm_f =  compute_tm prec ord I a f"
     apply(simp) using map_option_eq_Some by metis
-  have t_decomp: "t = tm_pow prec ord tm_f k I a"
+  have t_decomp: "t = tm_pow prec ord I a tm_f k"
     using Power(3) by (simp add: tm_f_def[symmetric])
   show ?case
     using tm_pow_valid[OF Power(1)[OF Power(2)[simplified] tm_f_def]]
@@ -1453,8 +1487,8 @@ next
   case (Inverse f t)
   from Inverse(3) obtain tf where tf_def: "Some tf = compute_tm prec ord I a f"
     by (simp, metis (no_types, lifting) option.case_eq_if option.collapse)
-  have "\<And>x. x \<in> set_of (interval_map real_of_float (compute_bound_tm tf I a)) \<Longrightarrow>
-          0 < lower (compute_bound_tm tf I a) \<or> upper (compute_bound_tm tf I a) < 0 \<Longrightarrow>
+  have "\<And>x. x \<in> set_of (interval_map real_of_float (compute_bound_tm I a tf)) \<Longrightarrow>
+          0 < lower (compute_bound_tm I a tf) \<or> upper (compute_bound_tm I a tf) < 0 \<Longrightarrow>
           isDERIV 0 (Inverse (Var 0)) [x]"
     by (simp add: set_of_def interval_map_def, safe, simp_all)
   thus ?case
@@ -1485,8 +1519,8 @@ next
   case (Ln f t)
   from Ln(3) obtain tf where tf_def: "Some tf = compute_tm prec ord I a f"
     by (simp, metis (no_types, lifting) option.case_eq_if option.collapse)
-  have "\<And>x. x \<in> set_of (interval_map real_of_float (compute_bound_tm tf I a)) \<Longrightarrow>
-          0 < lower (compute_bound_tm tf I a) \<Longrightarrow>
+  have "\<And>x. x \<in> set_of (interval_map real_of_float (compute_bound_tm I a tf)) \<Longrightarrow>
+          0 < lower (compute_bound_tm I a tf) \<Longrightarrow>
           isDERIV 0 (Ln (Var 0)) [x]"
     by (simp add: set_of_def interval_map_def)
   thus ?case
@@ -1496,8 +1530,8 @@ next
   case (Sqrt f t)
   from Sqrt(3) obtain tf where tf_def: "Some tf = compute_tm prec ord I a f"
     by (simp, metis (no_types, lifting) option.case_eq_if option.collapse)
-  have "\<And>x. x \<in> set_of (interval_map real_of_float (compute_bound_tm tf I a)) \<Longrightarrow>
-          0 < lower (compute_bound_tm tf I a) \<Longrightarrow>
+  have "\<And>x. x \<in> set_of (interval_map real_of_float (compute_bound_tm I a tf)) \<Longrightarrow>
+          0 < lower (compute_bound_tm I a tf) \<Longrightarrow>
           isDERIV 0 (Sqrt (Var 0)) [x]"
     by (simp add: set_of_def interval_map_def)
   thus ?case
@@ -1512,7 +1546,7 @@ next
 next
   case (Abs f t)
   from Abs(3) obtain tf where tf_def: "Some tf = compute_tm prec ord I a f"
-                        and  t_def: "t = tm_abs tf I a"
+                        and  t_def: "t = tm_abs I a tf"
     by (metis (no_types, lifting) compute_tm.simps(14) map_option_eq_Some)
   from tm_abs_valid[OF Abs(1)[OF Abs(2)[simplified] tf_def]]
   show ?case
@@ -1522,7 +1556,7 @@ next
   case (Min l r t)
   from Min(4)
   obtain t1 t2 where t_decomp:
-    "t = tm_min t1 t2 I a" and "Some t1 = compute_tm prec ord I a l" and "Some t2 = compute_tm prec ord I a r"
+    "t = tm_min I a t1 t2" and "Some t1 = compute_tm prec ord I a l" and "Some t2 = compute_tm prec ord I a r"
     by (smt compute_tm.simps(15) option.case_eq_if option.collapse option.distinct(2) option.inject split_conv)
   from this(2,3) Min(1-3)
   have t1_valid: "valid_tm I a (interpret_floatarith l) t1"
@@ -1541,7 +1575,7 @@ next
   case (Max l r t)
   from Max(4)
   obtain t1 t2 where t_decomp:
-    "t = tm_max t1 t2 I a" and "Some t1 = compute_tm prec ord I a l" and "Some t2 = compute_tm prec ord I a r"
+    "t = tm_max I a t1 t2" and "Some t1 = compute_tm prec ord I a l" and "Some t2 = compute_tm prec ord I a r"
     by (smt compute_tm.simps(16) option.case_eq_if option.collapse option.distinct(2) option.inject split_conv)
   from this(2,3) Max(1-3)
   have t1_valid: "valid_tm I a (interpret_floatarith l) t1"
@@ -1564,14 +1598,14 @@ subsection \<open>Computing bounds for floatarith expressions\<close>
 (* Automatically find interval bounds for floatarith expressions. *)
 fun compute_ivl_bound :: "nat \<Rightarrow> nat \<Rightarrow> float interval list \<Rightarrow> floatarith \<Rightarrow> float interval option"
 where "compute_ivl_bound prec n I f = (
-         map_option (\<lambda>t. round_ivl prec (compute_bound_tm t I (map mid I))) (compute_tm prec n I (map mid I) f)
+         map_option (\<lambda>t. round_ivl prec (compute_bound_tm I (map mid I) t)) (compute_tm prec n I (map mid I) f)
        )"
 
 (* Compute bounds using plain interval arithmetic by subdivision. *)
 fun compute_ivl_bound_naive :: "nat \<Rightarrow> nat \<Rightarrow> float interval list \<Rightarrow> floatarith \<Rightarrow> float interval option"
 where "compute_ivl_bound_naive prec n I f = (
          let Ds = split_domain (subdivide_interval n) I;
-             S = those (map (\<lambda>S. compute_bound prec f S) Ds)
+             S = those (map (\<lambda>S. compute_bound_fa prec f S) Ds)
          in map_option interval_list_union S
        )"
 
@@ -1583,7 +1617,7 @@ assumes "Some B = compute_ivl_bound prec n I f"
 assumes "x all_in I"
 shows "interpret_floatarith f x \<in> set_of B"
 proof-
-  from assms(3) obtain t where B_def: "B = round_ivl prec (compute_bound_tm t I (map mid I))" 
+  from assms(3) obtain t where B_def: "B = round_ivl prec (compute_bound_tm I (map mid I) t)" 
                            and t_def: "Some t = compute_tm prec n I (map mid I) f"
     by (smt compute_ivl_bound.simps map_option_eq_Some option.simps(8))
   
@@ -1609,7 +1643,7 @@ proof-
   then obtain i where i1: "i < length Ds"
              and i2: "x all_in (Ds ! i)"
     by (auto simp: Ds_def list_ex_length)
-  obtain S where S_def: "those (map (\<lambda>S. compute_bound prec f S) Ds) = Some S"
+  obtain S where S_def: "those (map (\<lambda>S. compute_bound_fa prec f S) Ds) = Some S"
     using assms(2) Ds_def
     by fastforce
   have "S \<noteq> []"
@@ -1626,14 +1660,14 @@ proof-
     using Some_those_length[OF S_def[symmetric]] i1
     by simp
   from Some_those_nth[OF S_def[symmetric] this]
-  have SomeSi: "Some (S ! i) = compute_bound prec f (Ds ! i)"
+  have SomeSi: "Some (S ! i) = compute_bound_fa prec f (Ds ! i)"
     by (simp add: i1)
   
   from Si_subset_B[OF \<open>i < length S\<close>]
   have "set_of (S ! i) \<subseteq> set_of (B::real interval)"
     by (simp add: interval_map_def set_of_def)
   thus ?thesis
-    using compute_bound_correct[OF i2 SomeSi]
+    using compute_bound_fa_correct[OF i2 SomeSi]
     by auto
 qed
 
