Experiments.thy
@@ -2,9 +2,8 @@ theory Experiments
 imports Taylor_Models
 begin
 
-(*
 (* Trying out arithmetic on intervals and polynomials with interval coefficients. *)
-value "Ivl (-1::float) 1 + Ivl 0 1"
+(*value "Ivl (-1::float) 1 + Ivl 0 1"
 value "Ivl (-8::float) 2 + Ivl (-2) (-1)"
 value "Ivl (0::real) 1 * Ivl 0 1"
 value "Ivl (-10::real) 6 * Ivl (-4) 2"
@@ -12,9 +11,9 @@ value "Ivl (-1::real) 1 * Ivl 0 1"
 value "Ivl (-1::float) 1 * Ivl 0 1"
 value "Ipoly [Ivl (Float 4 (-6)) (Float 10 (-6))] (poly.Add (poly.C (Ivl (Float 3 (-5)) (Float 3 (-5)))) (poly.Bound 0))"
 
-value "compute_bound 64 (Add (Var 0) (Num 3)) [Ivl 1 2]"
+value "compute_bound_fa 64 (Add (Var 0) (Num 3)) [Ivl 1 2]"
 
-value "map_option (interval_map real_of_float) (compute_bound 16 (Cos (Var 0)) [Ivl (-1) 1])"
+value "map_option (interval_map real_of_float) (compute_bound_fa 16 (Cos (Var 0)) [Ivl (-1) 1])"
 
 value "map (interval_map real_of_float) (the (tmf_cs 32 10 (Ivl 0 2) 1 (Cos (Var 0))))"
 
@@ -25,11 +24,11 @@ value "the (compute_tm 32 7 [Ivl 0 2, Ivl 0 2] [1,1] (Add (Var 0) (Var 1)))"
 value "tm_norm_poly (the (compute_tm 32 10 [Ivl (-1) 1] [0] (Cos (Var 0))))"
 value [code] "tm_norm_poly (the (compute_tm 32 7 [Ivl (-1) 1, Ivl (-1) 1] [0, 0] (Add (Exp (Add (Var 0) (Var 1))) (Cos (Mult (Var 0) (Var 1))))))"
 
-value "let I = [Ivl 1 3]; a = [2] in case (the (compute_tm 32 10 I a (Inverse (Var 0)))) of TaylorModel p e \<Rightarrow> (tm_lower_order (TaylorModel p e) 5 I a)"
+value "let I = [Ivl 1 3]; a = [2] in case (the (compute_tm 32 10 I a (Inverse (Var 0)))) of TaylorModel p e \<Rightarrow> (tm_lower_order 5 (TaylorModel p e) I a)"
 
 value "map_option (interval_map real_of_float) (compute_ivl_bound 32 10 [Ivl (-1) 1] (Power (Cos (Var 0)) 2))"
 value "map_option (interval_map real_of_float) (compute_ivl_bound 32 10 [Ivl (1) 2] (Inverse (Add (Cos (Var 0)) (Num 2))))"
-value "map_option (interval_map real_of_float) (compute_ivl_bound 32 10 [Ivl (1) 2] (Inverse (Var 0)))"
+value "map_option (interval_map real_of_float) (compute_ivl_bound 32 10 [Ivl (1) 2] (Inverse (Var 0)))"*)
 
 (*definition "test (u::unit) = prove_pos 50 40 (FloatR 1 (-3)) (FloatR 1 (-1)) caprasse (aform_of_ivl (mk_tuple4 (- FloatR 1 (-1))) (mk_tuple4 (FloatR 1 (-1))))"*)
 definition "test (u::unit) = the (compute_tm 32 7 [Ivl 0 2, Ivl 0 2] [1,1] (Add (Var 0) (Var 1)))"
@@ -37,9 +36,56 @@ definition "test (u::unit) = the (compute_tm 32 7 [Ivl 0 2, Ivl 0 2] [1,1] (Add 
 ML \<open>val test = @{code test}\<close>
 
 ML \<open>test ()\<close>
-ML \<open>Timing.timeit test\<close>*)
+ML \<open>Timing.timeit test\<close>
 
-value "the (compute_tm 32 10 [Ivl (-1) 1] [0] (Cos (Var 0)))"
+definition "approx_cos I = (case the (compute_tm 32 10 I (map mid I) (Cos (Var 0))) of TaylorModel p e \<Rightarrow> (p, e))"
+
+fun approx_cos_error
+where "approx_cos_error I = snd (approx_cos [Ivl (-1) 1])"
+
+fun approx_cos_naive
+where "approx_cos_naive I = Ipoly I (polynate (polysubst0 (poly.Sub (poly.Bound 0) (poly.C (mid (hd I)))) (fst (approx_cos I))))"
+
+fun approx_cos_trans
+where "approx_cos_trans I = Ipoly (list_op op- I (map mid I)) (fst (approx_cos I))"
+
+fun approx_cos_best
+where "approx_cos_best I = compute_bound_poly (fst (approx_cos I)) I (map mid I)"
+
+value "approx_cos_error [Ivl (-1) 1]"
+value "approx_cos_error [Ivl 1 3]"
+value "approx_cos_error [Ivl 3 5]"
+value "approx_cos_error [Ivl 5 7]"
+value "approx_cos_error [Ivl 7 9]"
+value "approx_cos_error [Ivl 9 11]"
+
+value "approx_cos_naive [Ivl (-1) 1]"
+value "approx_cos_naive [Ivl 1 3]"
+value "approx_cos_naive [Ivl 3 5]"
+value "approx_cos_naive [Ivl 5 7]"
+value "approx_cos_naive [Ivl 7 9]"
+value "approx_cos_naive [Ivl 9 11]"
+
+value "approx_cos_trans [Ivl (-1) 1]"
+value "approx_cos_trans [Ivl 1 3]"
+value "approx_cos_trans [Ivl 3 5]"
+value "approx_cos_trans [Ivl 5 7]"
+value "approx_cos_trans [Ivl 7 9]"
+value "approx_cos_trans [Ivl 9 11]"
+
+value "approx_cos_best [Ivl (-1) 1]"
+value "approx_cos_best [Ivl 1 3]"
+value "approx_cos_best [Ivl 3 5]"
+value "approx_cos_best [Ivl 5 7]"
+value "approx_cos_best [Ivl 7 9]"
+value "approx_cos_best [Ivl 9 11]"
+
+value "approx_cos_error [Ivl (-11) (-9)]"
+value "approx_cos_naive [Ivl (-11) (-9)]"
+value "approx_cos_trans [Ivl (-11) (-9)]"
+value "approx_cos_best [Ivl (-11) (-9)]"
+
+(*value "the (compute_tm 32 10 [Ivl (-1) 1] [0] (Cos (Var 0)))"
 value "the (compute_tm 32 10 [Ivl (-1) 1] [0] (Cos (Add (Var 0) (Mult (Num 2) Pi))))"
 value "the (compute_tm 32 10 [Ivl 9 11] [10] (Cos (Var 0)))"
 value "the (compute_tm 32 10 [Ivl (-10) 10] [0] (Cos (Var 0)))"
@@ -49,6 +95,7 @@ value "the (compute_tm 32 10 [Ivl 9 11] [10] (Add (Power (Cos (Var 0)) 2) (Power
 value "the (compute_tm 32 10 [Ivl (-1) 1] [0] (Add (Power (Cos (Add (Var 0) (Num (-2)))) 2) (Power (Sin (Add (Var 0) (Num (-2)))) 2)))"
 value "the (compute_tm 32 10 [Ivl 1 3] [2] (Add (Power (Cos (Add (Var 0) (Num (-2)))) 2) (Power (Sin (Add (Var 0) (Num (-2)))) 2)))"
 
+value "the (compute_ivl_bound 32 10 [Ivl (1000) 1002] (Cos (Var 0)))"
 value "the (compute_ivl_bound 32 10 [Ivl (-1) 1] (Cos (Var 0)))"
 value "the (compute_ivl_bound 32 10 [Ivl (-1) 1] (Cos (Add (Var 0) (Mult (Num 2) Pi))))"
 value "the (compute_ivl_bound 32 10 [Ivl 9 11] (Cos (Var 0)))"
@@ -57,6 +104,6 @@ value "the (compute_ivl_bound 32 10 [Ivl (-1) 1] (Add (Power (Cos (Var 0)) 2) (P
 value "the (compute_ivl_bound 32 10 [Ivl 1 3] (Add (Power (Cos (Var 0)) 2) (Power (Sin (Var 0)) 2)))"
 value "the (compute_ivl_bound 32 10 [Ivl 9 11] (Add (Power (Cos (Var 0)) 2) (Power (Sin (Var 0)) 2)))"
 value "the (compute_ivl_bound 32 10 [Ivl (Float (-1) (-4)) (Float (1) (-4))] (Add (Power (Cos (Add (Var 0) (Num (-2)))) 2) (Power (Sin (Add (Var 0) (Num (-2)))) 2)))"
-value "the (compute_ivl_bound 32 10 [Ivl 1 3] (Add (Power (Cos (Add (Var 0) (Num (-2)))) 2) (Power (Sin (Add (Var 0) (Num (-2)))) 2)))"
+value "the (compute_ivl_bound 32 10 [Ivl 1 3] (Add (Power (Cos (Add (Var 0) (Num (-2)))) 2) (Power (Sin (Add (Var 0) (Num (-2)))) 2)))"*)
 
 end
